pancake/panLangScript.sml
@@ -54,6 +54,7 @@ Datatype:
       | Cmp cmp exp exp
       | Shift shift exp num
       | BaseAddr
+      | TopAddr
       | BytesInWord
 End
 
